AbelianMonoid.v
@@ -11,34 +11,42 @@ Class Semigroup {A : Type} (op : A -> A -> A) : Type := {
   op_associative : forall x y z : A, op x (op y z) = op (op x y) z
 }.
 
-(** Monoid is a semigroup with left and right IDs *)
+(** A monoid is a semigroup with left and right identity values *)
 Class Monoid `(M : Semigroup) (id : A) : Type := {
   id_ident_left  : forall x : A, op id x = x;
   id_ident_right : forall x : A, op x id = x
 }.
 
-(** Abelian monoid is a monoid whose operator is commutative *)
+(** An abelian monoid is a monoid whose operator is commutative *)
 Class AbelianMonoid `(M : Monoid) : Type := {
   op_commutative : forall x y : A, op x y = op y x
 }.
 
-Instance ExSemigroup : (Semigroup mult) := {
+(** Let's explore multiplication as a semigroup, monoid and abelian monoid.
+  First, we'll show that multiplication is a semigroup by creating an instance
+  of [Semigroup] named [MultAsSemigroup]. *)
+
+Instance MultAsSemigroup : (Semigroup mult) := {
 }.
 Proof.
   intros. apply mult_assoc.
-Qed.
+Defined.
 
-Instance ExMonoid : (Monoid ExSemigroup 1) := {
+Instance MultAsMoioid2 : (Monoid (Semigroup mult) 1) := {
+}.
+
+Instance MultAsMonoid : (Monoid MultAsSemigroup 1) := {
 }.
 Proof.
   intros. apply mult_1_l.
   intros. apply mult_1_r.
-Qed.
+Defined.
 
-Instance ExAbMonoid : (AbelianMonoid ExMonoid) :=
+Instance MultAsAbelianMonoid : (AbelianMonoid MultAsMonoid) :=
 {
 }.
 Proof.
   intros. apply mult_comm.
-Qed.
+Defined.
 
+Quit.
